ems/Skeleton.v
@@ -43,7 +43,6 @@ Proof.
   - rewrite Heq0. specialize (IHl (S n)). rewrite Heq0 in IHl. ss.
 Qed.
 
-
 Module SkEnv.
 
   Class t: Type := mk {
@@ -59,12 +58,6 @@ Module SkEnv.
 
 End SkEnv.
 
-
-
-
-
-
-Require Import Orders.
 
 Module Sk.
   Class ld: Type := mk {
